src/LogRel.v
@@ -164,7 +164,8 @@ Section Tests.
     destruct H, H1. eapply H2; eauto. rewrite Vrel_Fix_eq. unfold e1, Vrel_rec. repeat constructor.
     apply length_zero_iff_nil in H3. apply length_zero_iff_nil in H4. subst. intros. cbn. cbn in H4.
     destruct H3, H6. epose (H7 m1 _ (ELit 0) (ELit 0) _ H4).
-    destruct t. exists (S (S (S x))). constructor. econstructor. constructor. assumption.
+    destruct t. exists (S (S (S x))). constructor. econstructor. constructor.
+    constructor. assumption.
     Unshelve.
     all: repeat constructor.
   Qed.
